이거, LinearDistinct 를 만들어야 할 것 같은데... - LinearBijection 이랑...?

src/common/Nemonuri.Bijective.IndexMap.fst
@@ -4,37 +4,13 @@ module I = FStar.IntegerIntervals
 module ISet = Nemonuri.IndexSet
 open Nemonuri.IndexMap { count, last_key, first_key, key_t, contained_data_t,
                          ensured_data_t, max_key,
-                         key_value, is_empty,
-                         interval_does_not_contain_value }
-open Nemonuri.IndexMap.Unique
+                         key_value_t, is_empty, lemma_push_pop, lemma_pop_push }
+open Nemonuri.IndexMap.Unique { map_is_distinct, unique_key_predicate, lemma_map_is_distinct,
+                                unique_key_t, unique_data_t }
 module IMap = Nemonuri.IndexMap
-module Seq = FStar.Seq.Base
-module List = FStar.List.Tot
-open FStar.Bijection { (=~) }
-module B = FStar.Bijection
+module Cl = FStar.Classical
 
-let interval_is_bijective (#data_t:eqtype) (m:IMap.t data_t) (min:key_t m) (imax:key_t m) =
-  forall (x:key_t m). (I.interval_condition min (imax+1) x) ==>
-    ((min = imax) <==> (IMap.select m min = IMap.select m imax))
-
-let bijective_index_map_predicate (#data_t:eqtype) (m:IMap.t data_t) =
-  forall (x:contained_data_t m). (unique_data_predicate m x)
-  //m |> IMap.to_seq |> Seq.seq_to_list |> List.noRepeats
-
-(*
-let lemma_bijective_index_map_predicate (#data_t:eqtype) (m:IMap.ensured_t data_t)
-  : Lemma ((interval_is_bijective m 0 (max_key m)) <==> (bijective_index_map_predicate m))
-  =
-  ()
-*)
-
-(*
-private let rec is_bijective_agg' 
-  (#data_t:eqtype) (m:IMap.t data_t) 
-  (asc_select_key:key_t m) (des_compare_key:key_t m{des_compare_key < asc_select_key})
-  =
-*)
-
+let bijective_index_map_predicate (#data_t:eqtype) (m:IMap.t data_t) = map_is_distinct m
 
 type t (data_t:eqtype) = x:IMap.t data_t{bijective_index_map_predicate x}
 
@@ -42,7 +18,7 @@ type ensured_t (data_t:eqtype) = x:t data_t{not (is_empty x)}
 
 let lemma_key #data_t (m:t data_t) (key:key_t m)
   : Lemma (unique_key_predicate m key) =
-  ()
+  lemma_map_is_distinct m
 
 let select #data_t (m:t data_t) (key:unique_key_t m) : Tot (unique_data_t m) = IMap.select m key
 let unique_key #data_t (m:t data_t) (v:unique_data_t m) : Tot (unique_key_t m) = IMap.first_key m v
@@ -50,34 +26,33 @@ let unique_key #data_t (m:t data_t) (v:unique_data_t m) : Tot (unique_key_t m) =
 
 let empty (#data_t:eqtype) (fb:data_t) : Tot (t data_t) = IMap.empty fb
 
-let fresh_data_predicate #data_t (m:t data_t) (v:ensured_data_t m) : Tot bool = not (IMap.contains_value m v)
-type fresh_data_t #data_t (m:t data_t) = x:ensured_data_t m{fresh_data_predicate m x}
+let fresh_data_predicate (#data_t:eqtype) (m:IMap.t data_t) (v:ensured_data_t m) : Tot bool = not (IMap.contains_value m v)
+type fresh_data_t (#data_t:eqtype) (m:IMap.t data_t) = x:ensured_data_t m{fresh_data_predicate m x}
 
-
-
-
-//let lemma_push_fresh_data_unique #data_t (m:t data_t) (v:fresh_data_t m)
-
-(*
-let pop #data_t (m:ensured_t data_t) : Tot ((t data_t) & (key_value data_t)) =
-  let ( m2, kv ) = IMap.pop m in
-  ( m2, kv )
-*)
+let lemma_fresh_data (#data_t:eqtype) (m:IMap.t data_t) (v:ensured_data_t m)
+  : Lemma (((bijective_index_map_predicate m) /\ (fresh_data_predicate m v)) <==>
+           (bijective_index_map_predicate (IMap.push m v)))
+  =
+  let pl = ((bijective_index_map_predicate m) /\ (fresh_data_predicate m v)) in
+  let pr = (bijective_index_map_predicate (IMap.push m v)) in
+  let lemma_pl_to_pr () : Lemma (requires pl) (ensures pr) =
+    admit ()
+  in
+  let lemma_pr_to_pl () : Lemma (requires pr) (ensures pl) =
+    admit ()
+  in
+  Cl.move_requires lemma_pl_to_pr ();
+  Cl.move_requires lemma_pr_to_pl ()
 
 let push #data_t (m:t data_t) (v:fresh_data_t m) 
   : Tot (t data_t) = 
-  let next_m = IMap.push m v in
-  assert (interval_does_not_contain_value next_m v 0 (count m));
-  assert (~(interval_does_not_contain_value next_m v 0 (count next_m)));
-  assert ((last_key next_m v) = (first_key next_m v));
-  assert (unique_data_predicate next_m v);
-  //assume (IMap.first_key next_m v = IMap.max_key next_m);
-  //assume (IMap.last_key next_m v = IMap.max_key next_m);
-  //assert (IMap.first_key next_m v = IMap.last_key next_m v);
-  //assume (forall (x:key_t m). (unique_key_predicate next_m x));
-  //assert (unique_data_predicate next_m v);
-  assume (bijective_index_map_predicate next_m);
-  next_m
-  
+  lemma_fresh_data m v;
+  IMap.push m v
+
+let pop #data_t (m:ensured_t data_t) : Tot ((t data_t) & (key_value_t data_t)) =
+  let ( m2, kv ) = IMap.pop m in
+  lemma_pop_push m;
+  ( m2, kv )
+
 
 
